concurrency/lifting.v
@@ -55,14 +55,8 @@ Module lifting.
         gS gT main
         ge_inv init_inv halt_inv.
     Proof.
-      eapply Build_Wholeprog_sim with (core_data:=unit).
     Admitted.
 
-(*    Lemma compiler_safety: forall n sch main ge1 ge2 p,
-        (genv_inv (concur_sim main sch ge1 ge2)).
-        initial_core (DMachineSem sch p) ge1 main vals1 = Some c1 ->
-        DryMachine.csafe *)
-        
   End lifting.
 End lifting.
       
